examples/crypto/cryptobox/Box.PKAE.fst
@@ -20,7 +20,7 @@ module HS = FStar.HyperStack
 
 type rid = FStar.Monotonic.Seq.rid
 
-assume val pkae_afternm_table_region: (r:MR.rid{ extends r root 
+assume val box_log_region: (r:MR.rid{ extends r root 
 					 /\ is_eternal_region r 
 					 /\ is_below r root 
 					 /\ disjoint r ae_key_region 
@@ -29,32 +29,32 @@ assume val pkae_afternm_table_region: (r:MR.rid{ extends r root
 					 /\ disjoint r id_freshness_table_region
 					 })
 
-assume val pkae_beforenm_table_region: (r:MR.rid{ extends r root 
+assume val box_key_log_region: (r:MR.rid{ extends r root 
 					 /\ is_eternal_region r 
 					 /\ is_below r root 
 					 /\ disjoint r ae_key_region 
 					 /\ disjoint r dh_key_log_region
 					 /\ disjoint r id_honesty_table_region
 					 /\ disjoint r id_freshness_table_region
-					 /\ disjoint r pkae_afternm_table_region
+					 /\ disjoint r box_log_region
 					 })
 					 
 //let pkae_table_region = new_region root
 
 
-type pkae_afternm_table_key = (nonce*(i:id{AE_id? i}))
-type pkae_afternm_table_value = (protected_pkae_plain)
-type pkae_afternm_table_range = fun pkae_afternm_table_key -> pkae_afternm_table_value
-type pkae_afternm_table_inv (f:MM.map' pkae_afternm_table_key pkae_afternm_table_range) = True
-assume val pkae_afternm_table: MM.t pkae_afternm_table_region pkae_afternm_table_key pkae_afternm_table_range pkae_afternm_table_inv
-//let pkae_afternm_table = MM.alloc #pkae_table_region #pkae_table_key #pkae_table_range #pkae_table_inv
+type box_log_key = (nonce*(i:id{AE_id? i /\ honest i}))
+type box_log_value = (protected_pkae_plain)
+type box_log_range = fun box_log_key -> box_log_value
+type box_log_inv (f:MM.map' box_log_key box_log_range) = True
+assume val box_log: MM.t box_log_region box_log_key box_log_range box_log_inv
+//let box_log = MM.alloc #pkae_table_region #pkae_table_key #pkae_table_range #pkae_table_inv
 
-type pkae_beforenm_table_key = i:id{AE_id? i}
-type pkae_beforenm_table_value = (AE.key)
-type pkae_beforenm_table_range = fun (i:pkae_beforenm_table_key) -> (k:pkae_beforenm_table_value{AE.get_index k = i})
-type pkae_beforenm_table_inv (f:MM.map' pkae_beforenm_table_key pkae_beforenm_table_range) = True
-assume val pkae_beforenm_table:  MM.t pkae_beforenm_table_region pkae_beforenm_table_key pkae_beforenm_table_range pkae_beforenm_table_inv
-//let pkae_beforenm_table = MM.alloc #pkae_table_region #pkae_table_key #pkae_table_range #pkae_table_inv
+type box_key_log_key = i:id{AE_id? i /\ honest i}
+type box_key_log_value = (AE.key)
+type box_key_log_range = fun (i:box_key_log_key) -> (k:box_key_log_value{AE.get_index k = i})
+type box_key_log_inv (f:MM.map' box_key_log_key box_key_log_range) = True
+assume val box_key_log:  MM.t box_key_log_region box_key_log_key box_key_log_range box_key_log_inv
+//let box_key_log = MM.alloc #pkae_table_region #pkae_table_key #pkae_table_range #pkae_table_inv
 
 
 noeq abstract type pkae_pkey (pk_id:id{DH_id? pk_id}) =
@@ -66,7 +66,7 @@ noeq abstract type pkae_skey (sk_id:id{DH_id? sk_id}) =
 val keygen: #(i:id{DH_id? i}) -> ST (pkae_pkey i * pkae_skey i)
   (requires (fun h0 -> 
   fresh i h0
-  /\ fixed i
+  /\ registered i
   ))
   (ensures (fun h0 res h1 -> 
     unfresh i
@@ -80,105 +80,96 @@ let keygen #i =
 
 type c = AE.cipher
 
-// Need to remodel the invariant. We cannot guarantee points two and three in the face of multiple (dishonest) keys with the same id.
+// TODO: We should be able to replace "dishonest i"  with "~(honest i)" everywhere!
 let log_invariant (h:mem) = 
-  (forall (k:AE.key). let i = AE.get_index k in ~( fresh i h))
-  /\
-  (forall (i:id{AE_id? i}) (n:nonce). fresh i h ==> MM.fresh pkae_afternm_table (n,i) h)
-  /\
-  (forall (k:AE.key) (n:nonce). let k_log = get_logGT k in (MM.fresh k_log n h <==> MM.fresh pkae_afternm_table (n,AE.get_index k) h))
-  //forall (k:AE.key) (n:nonce). let k_log = get_logGT k in ( (MM.fresh k_log n h <==> MM.fresh pkae_afternm_table (n,AE.get_index k) h) /\ ( (MR.m_sel h k_log == MM.empty_map AE.log_key (AE.log_range (AE.get_index k))) <==> MM.fresh pkae_afternm_table (n,AE.get_index k) h) )
+  (forall (i:id{AE_id? i /\ honest i}) .(*{:pattern (MM.defined box_key_log i h) \/ (honest i /\ AE_id? i) \/ (MM.defined dh_key_log i h)}*) MM.defined box_key_log i h <==> MM.defined dh_key_log i h) // dh_key_log and box_key_log are in sync
+  ///\ 
+  //(forall (i:id{AE_id? i /\ honest i}) . MM.fresh box_key_log i h <==> fresh i h)
+  ///\
+  //(forall (i:id{AE_id? i /\ honest i}) (n:nonce) . (MM.defined box_key_log i h ==> (let k = MM.value box_key_log i h in 
+  //									   let k_log = get_logGT k in
+  //									   MM.defined box_log (n,i) h <==> MM.defined k_log n h)))
+  ///\
+  //(forall (i:id{AE_id? i /\ honest i}) (n:nonce) . (MM.fresh box_key_log i h ==> MM.fresh box_log (n,i) h))
 
 
 
-//val invariant_lemma: (h0:mem) -> k:AE.key ->  h1:mem -> Lemma
-//  (requires (
-//    log_invariant h0
-//    /\ (forall (k':AE.key).{:pattern (MR.m_sel h1 (get_logGT k'))} let k_log = get_logGT k' in (~(k == k') ==> MR.m_sel h0 k_log == MR.m_sel h1 k_log) /\ (( k == k') ==> (MR.m_sel h1 k_log == MM.empty_map AE.log_key (AE.log_range (AE.get_index k)))))
-//    /\ MR.m_sel h0 pkae_afternm_table == MR.m_sel h1 pkae_afternm_table
-//    /\ (forall (n:nonce) . (MM.fresh pkae_afternm_table (n,AE.get_index k) h0))
-//  ))
-//  (ensures (log_invariant h1))
-//let invariant_lemma h0 k h1 = ()
-
-
-// Make sure that if the key is fresh, then there is no entry in the pkae_afternm_table.
-// Maybe do this by connecting with the id_freshness_table?
 #set-options "--z3rlimit 25"
-val encrypt_beforenm: #(pk_id:id{DH_id? pk_id /\ fixed pk_id}) -> 
-	              #(sk_id:id{DH_id? sk_id /\ fixed sk_id}) -> 
+val encrypt_beforenm: #(pk_id:id{DH_id? pk_id /\ registered pk_id}) -> 
+	              #(sk_id:id{DH_id? sk_id /\ registered sk_id}) -> 
 	              pk:pkae_pkey pk_id -> 
 	              sk:pkae_skey sk_id ->
 		      ST (k:AE.key)
   (requires (fun h0 -> 
     let i = generate_ae_id pk_id sk_id in
-    fixed i
-    /\ ((honest i /\ MM.fresh dh_key_log i h0) ==> (fresh i h0))
+    registered i
+    /\ (honest i /\ MM.fresh box_key_log i h0 ==> fresh i h0)
     /\ log_invariant h0
   ))
   (ensures (fun h0 k h1 -> 
     let i = generate_ae_id pk_id sk_id in
-    let regions_modified_dishonest:Set.set (r:HH.rid) = (Set.singleton id_freshness_table_region) in
-    let regions_modified_honest = Set.union regions_modified_dishonest (Set.singleton dh_key_log_region) in
+    let regions_modified_dishonest = [id_freshness_table_region] in
+    let regions_modified_honest_set = Set.as_set (regions_modified_dishonest @ [dh_key_log_region;box_key_log_region]) in
+    let regions_modified_dishonest_set:Set.set (r:HH.rid) = Set.as_set regions_modified_dishonest in
     let k_log = get_logGT k in
     (PlainDH.ae_key_get_index k = i)
     /\ (
         ( (honest i)
-    	    ==> (modifies regions_modified_honest h0 h1
-    	       /\ MR.witnessed (MM.contains dh_key_log i k) 
-    	      )
+    	    ==> (modifies regions_modified_honest_set h0 h1
+    	       /\ (MR.witnessed (MM.contains dh_key_log i k) 
+		 \/ MR.witnessed (MM.contains box_key_log i k)
+    		 )
+	      )
         )
         \/ 
     	( (dishonest i \/ ~Flags.prf_odh)
-    	    ==> (modifies regions_modified_dishonest h0 h1
+    	    ==> (modifies regions_modified_dishonest_set h0 h1
     	       /\ leak_key k = DH.prf_odhT sk.dh_sk pk.dh_pk
     	      )
         )
       )
     /\ MR.m_contains k_log h1
-    /\ modifies regions_modified_honest h0 h1
-    /\ (forall k. let k_region = get_regionGT k in
-      equal_on (Set.singleton k_region) h0.h h1.h)
-    /\ (let k_region = get_regionGT k in
-      equal_on (Set.singleton pkae_afternm_table_region) h0.h h1.h)
-    ///\ log_invariant h1
+    /\ modifies regions_modified_honest_set h0 h1
+    /\ (forall (i:id{AE_id? i /\ honest i}) . MM.defined box_key_log i h1 <==> MM.defined dh_key_log i h1)
+    ///\ (forall (i:id{AE_id? i /\ honest i}) (n:nonce) . MM.defined box_key_log i h ==> (let k = MM.value box_key_log i h in 
+	//								   let k_log = get_logGT k in
+		//							   MM.defined box_log (n,i) h <==> MM.defined k_log n h))
+    /\ log_invariant h1
   ))
 let encrypt_beforenm #pk_id #sk_id pk sk =
-  MR.m_recall pkae_afternm_table;
-  let h0 = ST.get() in
-  assert(log_invariant h0);
-  let k = prf_odh sk.dh_sk pk.dh_pk in
-  let h1 = ST.get() in
-  assert(forall (i:id). ~(fresh i h0) ==> ~(fresh i h1));
-  assert(forall (i:id{AE_id? i}) (n:nonce). fresh i h1 ==> MM.fresh pkae_afternm_table (n,i) h1);
-  assert(forall (k:AE.key) . let i = AE.get_index k in let k_log = get_logGT k in fresh i h0 ==> (MR.m_sel h1 k_log == AE.empty_log i));
-  assert(forall (k:AE.key) . let i = AE.get_index k in ~( fresh i h1));
-  assert(forall (k:AE.key) (n:nonce) . let k_log = get_logGT k in MM.fresh k_log n h0 ==> MM.fresh k_log n h1);
-  //assert(forall (k:AE.key) (n:nonce). let k_log = get_logGT k in (MM.fresh k_log n h1 <==> MM.fresh pkae_afternm_table (n,AE.get_index k) h1));
-  //assume(forall (k':AE.key).{:pattern (MR.m_sel h1 (get_logGT k'))} let k_log = get_logGT k' in (~(k == k') ==> MR.m_sel h0 k_log == MR.m_sel h1 k_log) /\ (( k == k') ==> (MR.m_sel h1 k_log == MM.empty_map AE.log_key (AE.log_range (AE.get_index k)))));
-  //assert(log_invariant h1);
-  admit();
-  //assert(equal_on (Set.union (Set.singleton ae_key_region) (Set.singleton pkae_afternm_table_region)) h0.h h1.h);
-  assert(forall n.let k_log = get_logGT k in (MM.fresh k_log n h1 <==> MM.fresh pkae_afternm_table (n,AE.get_index k) h1));
-  admit();
-  recall_log k;
-  //let h0 = ST.get() in
-  //assert(log_invariant h0);
-  //admit();
-  k
+  MR.m_recall box_log;
+  MR.m_recall box_key_log;
+  MR.m_recall dh_key_log;
+  let i = generate_ae_id pk_id sk_id in
+  if is_honest i then
+    match MM.lookup box_key_log i with
+    | Some k -> 
+        recall_log k;
+        k
+    | None ->
+        let k = prf_odh sk.dh_sk pk.dh_pk in
+	MR.testify (MM.contains dh_key_log i k);
+        MM.extend box_key_log i k;
+	fresh_unfresh_contradiction i;
+        recall_log k;
+        k
+  else (
+    lemma_dishonest_not_honest i;
+    let k = prf_odh sk.dh_sk pk.dh_pk in
+    recall_log k;
+    k)
+  
 
 
-// Implement invariant that states equality of logs before and after encrypt_afternm.
-//   - quantify over all nonces and prove that lookups on both logs result in the same values.
 val encrypt_afternm: k:AE.key ->
 		     n:nonce ->
 		     p:protected_pkae_plain{PlainPKAE.get_index p = AE.get_index k} ->
 		     ST c
   (requires (fun h0 -> 
     let k_log = get_logGT k in
-    MM.fresh pkae_afternm_table (n,AE.get_index k) h0
+    MM.fresh box_log (n,AE.get_index k) h0
     /\ MR.m_contains k_log h0
-    /\ MR.m_contains pkae_afternm_table h0
+    /\ MR.m_contains box_log h0
     /\ log_invariant h0
   ))
   (ensures (fun h0 c h1 -> 
@@ -194,7 +185,7 @@ val encrypt_afternm: k:AE.key ->
     //  )
     (dishonest i \/ honest i)
     /\ MR.witnessed (MM.contains k_log n (c,ae_message_wrap p))
-    /\ MR.witnessed (MM.contains pkae_afternm_table (n,i) p)
+    /\ MR.witnessed (MM.contains box_log (n,i) p)
     /\ log_invariant h0
   ))
 let encrypt_afternm k n p =
@@ -205,26 +196,26 @@ let encrypt_afternm k n p =
 //  admit();
   let ae_i = AE.get_index k in
   let ae_m = ae_message_wrap #ae_i p in
-  MM.extend pkae_afternm_table (n,ae_i) p;
+  MM.extend box_log (n,ae_i) p;
   AE.encrypt #ae_i n k ae_m
   
 
 #set-options "--z3rlimit 25"
 val encrypt: #(pk_id:id{DH_id? pk_id}) -> 
 	     #(sk_id:id{DH_id? sk_id}) -> 
-	     pk:pkae_pkey pk_id{fixed pk_id} -> 
-	     sk:pkae_skey sk_id{fixed sk_id} -> 
+	     pk:pkae_pkey pk_id{registered pk_id} -> 
+	     sk:pkae_skey sk_id{registered sk_id} -> 
 	     n:nonce -> 
 	     p:protected_pkae_plain{PlainPKAE.get_index p = generate_ae_id pk_id sk_id} 
 	     -> ST unit
   (requires (fun h0 ->
     let i = generate_ae_id pk_id sk_id in
-    fixed i
-    /\ MR.m_contains pkae_afternm_table h0
+    registered i
+    /\ MR.m_contains box_log h0
     /\ (honest i ==> (~(MR.witnessed(MM.defined dh_key_log i) ==> ~(fresh i h0))))
-    /\ MM.fresh pkae_afternm_table (n,i) h0
+    /\ MM.fresh box_log (n,i) h0
     // Make sure that log_invariant holds
-    /\ MM.fresh pkae_afternm_table (n,i) h0
+    /\ MM.fresh box_log (n,i) h0
     /\ log_invariant h0
   ))
   (ensures (fun h0 c h1 -> 
@@ -249,7 +240,7 @@ val decrypt: #(sk_id:id) ->
 	     St(option (p:protected_pkae_plain))
 	     
 let decrypt #sk_id #pk_id n sk pk c =
-  MR.m_recall pkae_afternm_table;
+  MR.m_recall box_log;
   let (dh_sh,ae_c) = c in 
   let k = prf_odh sk.dh_sk pk.dh_pk  in
   let ae_i = AE.get_index k in
